secure_api/box/Box.Key.fst
@@ -1,136 +1,58 @@
-(**
-   This module exists to provide type information and functions needed by Box.DH. Box.AE is not imported directly by
-   Box.DH to preserve some notion of modularity. If Box.DH should be used with some other module, only Box.PlainDH
-   should have to be edited.
-*)
 module Box.Key
 
-open FStar.HyperHeap
 open FStar.HyperStack
 open FStar.HyperStack.ST
-open Crypto.Symmetric.Bytes
 
-open Box.Flags
+open FStar.Endianness
+open Box.Index
 
-module ID = Box.Index
-module Plain = Box.Plain
-module MR = FStar.Monotonic.RRef
-module HH = FStar.HyperHeap
-module HS = FStar.HyperStack
-module MM = MonotoneMap
-module SPEC = Spec.SecretBox
-
-assume val is_random: bytes -> Type0
-
-let index_module = ID.index_module
-let plain_module = Plain.plain_module
-let id = ID.id
-
-type log_region =
-  r:MR.rid{is_eternal_region r}
-
-type key_t (im:index_module) (pm:plain_module)= Type0
-
-//type aes_key = SPEC.key
-//type cipher = b:bytes{Seq.length b >= 16 /\ (Seq.length b - 16) / Spec.Salsa20.blocklen < pow2 32}
-//noeq type key_t2 (im:index_module) =
+// Definition KEY package
+noeq type key_package (#rgn:erid) (ip:index_package rgn) (key_length:(n:nat{n<=32})) (key_type:(inst_id  -> Type0)) =
+  | KP:
+  flag: Type0 ->
+  getGT: (#i:inst_id -> k:key_type i -> GTot (lbytes key_length)) ->
+  leak: (#i:inst_id{dishonest ip i \/ ~flag} -> k:key_type i -> (raw:lbytes key_length{raw = getGT k})) ->
+  gen: (i:inst_id -> k:key_type i) ->
+  coerce: (i:inst_id{~flag \/ dishonest ip i} -> raw:lbytes key_length -> (k:key_type i{raw = getGT k})) ->
+  key_package #rgn ip key_length key_type
 
 #set-options "--z3rlimit 300 --max_ifuel 1 --max_fuel 0"
-abstract noeq type key_module (im:index_module) =
-  | KM:
-    keylen: nat ->
-    key_type: (im':index_module{im' == im} -> t:Type0) ->
-    get_index: (k:key_type im -> i:id im) -> // You have to have faith in this function...
-    get_rawGT: ((k:key_type im) -> GTot (b:lbytes keylen)) -> // You have to have faith in this function...
-    invariant: (h:mem -> Type0) ->
-    key_log_region: (rgn:log_region{disjoint rgn (ID.get_rgn im)}) ->
-    gen: (i:id im -> ST (k:key_type im{get_index k = i}) // The spec should indicate that the result is random and that gen is idempotent
-      (requires (fun h0 ->
-        (ID.fresh im i h0 \/ ID.honest im i)
-        /\ invariant h0))
-      (ensures  (fun h0 k h1 ->
-        invariant h1
-        /\ modifies (Set.singleton key_log_region) h0 h1
-        ))) ->
-    set: ((i:id im {Game3? current_game \/ Game0? current_game}) -> (b:lbytes keylen) -> (k:key_type im{get_index k = i /\ b = get_rawGT k})) ->
-    coerce: (i:id im{ID.dishonest im i} -> raw:lbytes keylen -> (k:key_type im{get_index k = i /\ raw=get_rawGT k})) ->
-    leak: (k:key_type im{ID.dishonest im (get_index k)} -> (raw:lbytes keylen{raw = get_rawGT k})) ->
-    key_module im
+//val hon: (#inst_id:eqtype) -> (#key_length:(n:nat{n<=32})) -> (#key_type:(inst_id -> Type0)) -> kp:key_package #inst_id key_length key_type -> (kp_hon:(#i:inst_id -> key_type i -> bool){forall i . kp_hon #i === kp.hon #i})
+//let hon #inst_id #key_length #key_type kp = kp.hon
+//
+//val getGT: (#inst_id:eqtype) -> (#key_length:(n:nat{n<=32})) -> (#key_type:(inst_id -> Type0)) -> kp:key_package #inst_id key_length key_type -> (kp_getGT:(#i:inst_id -> k:key_type i -> GTot (lbytes key_length)){kp_getGT == kp.getGT})
+//let getGT #inst_id #key_length #key_type kp = kp.getGT
+//
+//val cget: (#inst_id:eqtype) -> (#key_length:(n:nat{n<=32})) -> (#key_type:(inst_id -> Type0)) -> kp:key_package #inst_id key_length key_type -> (#i:inst_id -> k:key_type i{kp.hon i k = false} -> (raw:lbytes key_length{raw = kp.getGT i k}))
+//let cget #inst_id #key_length #key_type kp = kp.cget
+//
+//val get: (#inst_id:eqtype) -> (#key_length:(n:nat{n<=32})) -> (#key_type:(inst_id -> Type0)) -> kp:key_package #inst_id key_length key_type -> (#i:inst_id -> k:key_type i -> (raw:lbytes key_length{raw = kp.getGT i k}))
+//
+//val gen: (#inst_id:eqtype) -> (#key_length:(n:nat{n<=32})) -> (#key_type:(inst_id -> Type0)) -> kp:key_package #inst_id key_length key_type -> (#i:inst_id -> k:key_type i{kp.hon i k = true})
+//let gen #inst_id #key_length #key_type kp = kp.gen
+//
+//val cset: (#inst_id:eqtype) -> (#key_length:(n:nat{n<=32})) -> (#key_type:(inst_id -> Type0)) -> kp:key_package #inst_id key_length key_type -> (#i:inst_id -> raw:lbytes key_length -> (k:key_type i{raw = kp.getGT i k /\ kp.hon i k = false}))
+//let cset #inst_id #key_length #key_type kp = kp.cset
 
-val get_keylen: im:index_module -> km:key_module im -> n:nat{n = km.keylen}
-let get_keylen im km =
-  km.keylen
-
-val get_keytype: im:index_module -> km:key_module im -> t:Type0{t == km.key_type im}
-let get_keytype im km =
-  km.key_type im
-
-val get_index: im:index_module -> km:key_module im -> gi:(k:km.key_type im -> i:id im){gi==km.get_index}
-let get_index im km =
-  km.get_index
-
-val get_rawGT: im:index_module -> km:key_module im -> gr:(k:km.key_type im -> GTot (b:lbytes km.keylen)){gr == km.get_rawGT}
-let get_rawGT im km =
-  km.get_rawGT
-
-val get_log_region: im:index_module -> km:key_module im -> rgn:log_region{rgn = km.key_log_region}
-let get_log_region im km =
-  km.key_log_region
-
-val gen: (im:index_module) -> (km:key_module im) -> (i:id im) -> ST (k:km.key_type im{km.get_index k = i})
-  (requires (fun h0 ->
-    (ID.fresh im i h0 \/ ID.honest im i)
-    /\ km.invariant h0))
-  (ensures  (fun h0 k h1 ->
-    km.invariant h1
-    /\ modifies (Set.singleton km.key_log_region) h0 h1
-  ))
-let gen im km i =
-  km.gen i
-
-val set: (im:index_module) -> (km:key_module im) -> (i:id im {~(Game2? current_game)}) -> (b:lbytes km.keylen) -> (k:km.key_type im{km.get_index k = i /\ b = km.get_rawGT k})
-let set im km i b =
-  km.set i b
-
-val coerce: (im:index_module) -> (km:key_module im) -> (i:id im{ID.dishonest im i}) -> (b:lbytes km.keylen) -> (k:km.key_type im{km.get_index k = i /\ b = km.get_rawGT k})
-let coerce im km i b =
-  km.coerce i b
-
-val leak: im:index_module -> (km:key_module im) -> (k:km.key_type im{ID.dishonest im (km.get_index k)}) -> (b:lbytes km.keylen{b=km.get_rawGT k})
-let leak im km k =
-  km.leak k
-
-val invariant: im:index_module -> km:key_module im -> inv:(h0:mem -> Type0){inv == km.invariant}
-let invariant im km =
-  km.invariant
-
-#set-options "--z3rlimit 2000 --max_ifuel 2 --max_fuel 0"
-val create: (im:index_module) ->
-            (keylen: nat) ->
-            (km_key_type: (im':index_module{im' == im} -> t:Type0)) ->
-            (km_get_index: (k:km_key_type im -> i:id im)) -> // You have to have faith in this function...
-            (km_get_rawGT: ((k:km_key_type im) -> GTot (b:lbytes keylen))) -> // You have to have faith in this function...
-            (km_invariant: (h:mem -> Type0)) ->
-            (km_key_log_region: (r:log_region{disjoint r (ID.get_rgn im)})) ->
-            (km_gen: (i:id im -> ST (k:km_key_type im{km_get_index k = i}) // The spec should indicate that the result is random and that gen is idempotent
-              (requires (fun h0 ->
-                (ID.fresh im i h0 \/ ID.honest im i)
-                /\ km_invariant h0))
-              (ensures  (fun h0 k h1 ->
-                km_invariant h1
-                /\ modifies (Set.singleton km_key_log_region) h0 h1
-              )))) ->
-            (km_set: (i:id im {Game3? current_game \/ Game0? current_game} -> b:lbytes keylen -> (k:km_key_type im{km_get_index k = i /\ b = km_get_rawGT k}))) ->
-            (km_coerce: (i:id im{ID.dishonest im i} -> raw:lbytes keylen -> (k:km_key_type im{km_get_index k = i /\ raw=km_get_rawGT k}))) ->
-            (km_leak: (k:km_key_type im{ID.dishonest im (km_get_index k)} -> (raw:lbytes keylen{raw = km_get_rawGT k}))) ->
-            (km:key_module im{
-              get_keytype im km == km_key_type im
-              /\ get_keylen im km == keylen
-              /\ get_index im km == km_get_index
-              /\ get_rawGT im km == km_get_rawGT
-              /\ invariant im km == km_invariant
-              /\ get_log_region im km == km_key_log_region
-    })
-let create im keylen km_key_type km_get_index km_get_rawGT km_invariant km_key_log_region km_gen km_set km_coerce km_leak =
-  let km = KM keylen km_key_type km_get_index km_get_rawGT km_invariant km_key_log_region km_gen km_set km_coerce km_leak in
-  km
+#set-options "--z3rlimit 300 --max_ifuel 1 --max_fuel 0"
+val create_key_package:
+  (#rgn:erid) ->
+  (ip:index_package rgn) ->
+  (flag:Type0) ->
+  (key_length:(n:nat{n<=32})) ->
+  (key_type:(inst_id -> Type0)) ->
+  (param_getGT: (#i:inst_id -> k:key_type i -> GTot (lbytes key_length))) ->
+  (param_leak: (#i:inst_id{dishonest ip i \/ ~flag} -> k:key_type i -> (raw:lbytes key_length{raw = param_getGT k}))) ->
+  (param_gen: (i:inst_id -> k:key_type i)) ->
+  (param_coerce: (i:inst_id{dishonest ip i \/ ~flag} -> raw:lbytes key_length -> (k:key_type i{raw = param_getGT k}))) ->
+  (kp:key_package #rgn ip key_length key_type{True
+//    param_hon == hon kp
+//    /\ param_hon == kp.hon
+//    /\ param_getGT == kp.getGT
+//    /\ param_getGT == getGT kp
+//    /\ param_cget == cget kp
+//    /\ param_gen == gen kp
+//    /\ param_cset == cset kp
+  })
+let create_key_package #rgn ip flag key_length key_type getGT leak gen coerce =
+  KP flag getGT leak gen coerce
