secure_api/box/Box.PKAE.fsti
@@ -1,171 +1,140 @@
 module Box.PKAE
 
-
 open FStar.Set
-open FStar.HyperHeap
+open FStar.Seq
 open FStar.HyperStack
 open FStar.HyperStack.ST
-open FStar.Monotonic.RRef
-open FStar.Seq
-open FStar.Monotonic.Seq
-open FStar.List.Tot
 
-open Crypto.Symmetric.Bytes
+open FStar.Endianness
 
-open Box.Flags
+open Box.Plain
+open Box.Index
 
-module MR = FStar.Monotonic.RRef
-module MM = MonotoneMap
-module HS = FStar.HyperStack
-module HH = FStar.HyperHeap
-module Plain = Box.Plain
-module ID = Box.Index
+module MM = FStar.Monotonic.Map
 
+let n32 = (n:nat{n<=32})
+let bytes32 = b:bytes{Seq.length b <= 32}
 
-val nonce: t:Type0{hasEq t}
-val cipher: Type0
-val sub_id: t:Type0{hasEq t}
-val key_id: Type0
-val plain: Type0
+val random_bytes: (n:n32) -> unit -> lbytes n
 
-val valid_plain_length: nat -> bool
-val valid_cipher_length: nat -> bool
+val pkae_flag: bool
 
-let index_module = im:ID.index_module{ID.id im == sub_id}
-let plain_index_module = im:ID.index_module{ID.id im == key_id}
+#set-options "--z3rlimit 300 --max_ifuel 1 --max_fuel 1"
 
-let log_region =
-  r:MR.rid{is_eternal_region r}
+val valid_length: nat -> bool
 
-val aux_t: (im:index_module) -> (kim:plain_index_module) -> (pm:Plain.plain_module) -> (rgn:log_region) -> Type u#1
+val pp : (pp:plain_package{pp.flag == b2t pkae_flag})
 
-abstract noeq type pkae_module =
-  | PKAE:
-    im:ID.index_module{ID.id im == sub_id} ->
-    pim:ID.index_module{ID.id pim == key_id} ->
-    pm:Plain.plain_module{Plain.get_plain pm == plain /\ Plain.valid_length #pm == valid_plain_length} ->
-    rgn:log_region ->
-//    enc: (plain -> n:nonce -> pk:pkey -> sk:skey{compatible_keys sk pk} -> GTot cipher) ->
-//    dec: (c:cipher -> n:nonce -> pk:pkey -> sk:skey{compatible_keys sk pk} -> GTot (option plain)) ->
-    aux: aux_t im pim pm rgn ->
-    pkae_module
+// Footpring function instead of rgn in the type
+val pkae_package: rgn:erid -> Type
 
-val skey: pkae_module -> Type0
-val pkey: pkae_module -> Type0
-
-val pkey_from_skey: (pkm:pkae_module -> sk:skey pkm -> pk:pkey pkm)
-
-val compatible_keys: (pkm:pkae_module -> sk:skey pkm -> pk:pkey pkm -> t:Type0{t <==> pk =!= pkey_from_skey pkm sk})
-
-val enc (pkm:pkae_module): plain -> n:nonce -> pk:pkey pkm -> sk:skey pkm{compatible_keys pkm sk pk} -> GTot cipher
-val dec (pkm:pkae_module): c:cipher -> n:nonce -> pk:pkey pkm -> sk:skey pkm{compatible_keys pkm sk pk} -> GTot (option plain)
-
-val compose_ids: pkae:pkae_module ->  s1:sub_id -> s2:sub_id{s2 <> s1} -> key_id
-
-val length: pkae:pkae_module -> p:plain -> n:nat{valid_plain_length n}
-
-
-
-type message_log_key (im:plain_index_module) = (nonce*(i:ID.id im))
-type message_log_value (im:plain_index_module) (i:ID.id im) = (cipher*Plain.protected_plain_t im plain i)
-type message_log_range (im:plain_index_module) (k:message_log_key im) = (v:message_log_value im (snd k))
-type message_log_inv (im:plain_index_module) (f:MM.map' (message_log_key im) (message_log_range im)) = True //t:Type0{t = True}
-type message_log (im:plain_index_module) (rgn:log_region) =
-  MM.t rgn (message_log_key im) (message_log_range im) (message_log_inv im)
-
-
-val get_message_log_region: pkm:pkae_module -> Tot (lr:log_region{extends lr pkm.rgn})
-val get_message_logGT: pkm:pkae_module -> Tot (message_log pkm.pim (get_message_log_region pkm)) //TODO: MK: would prefer this to be GTot
-
-val create: rgn:rid -> St (pkm:pkae_module)
-
-val zero_bytes: (n:nat{valid_plain_length n}) -> plain //b:bytes{Seq.length b = n /\ b=Seq.create n (UInt8.uint_to_t 0)}
-//TODO: MK this can be modelled better
-
-val pkey_to_subId: #pkm:pkae_module -> pk:pkey pkm -> ID.id pkm.im
-val pkey_to_subId_inj: #pkm:pkae_module -> pk:pkey pkm -> Lemma
-  (requires True)
-  (ensures (forall pk' . pkey_to_subId #pkm pk == pkey_to_subId #pkm pk' <==> pk == pk'))
-  [SMTPat (pkey_to_subId #pkm pk)]
-
-#set-options "--z3rlimit 2000 --max_ifuel 1 --max_fuel 0"
-val nonce_is_fresh: (pkm:pkae_module) -> (i:ID.id pkm.pim) -> (n:nonce) -> (h:mem) ->
-  (t:Type0{t <==>
-    (MR.m_contains #(get_message_log_region pkm) (get_message_logGT pkm) h
-      /\ MM.fresh #(get_message_log_region pkm)(get_message_logGT pkm) (n,i) h)})
-
-
-//val pkey_from_skey_inj: sk:skey -> pk:pkey -> Lemma
-//  (requires True)
-//  (ensures (forall sk1 sk2 . pkey_from_skey sk1 == pkey_from_skey sk2 <==> sk1 == sk2))
-
-val invariant: pkae_module -> mem -> Type0
-
-val gen: pkm:pkae_module -> ST (keypair:(pkey pkm*skey pkm){fst keypair == pkey_from_skey pkm (snd keypair)})
+val create_pkae_package: rgn:erid -> ST (pkae_package rgn)
   (requires (fun h0 -> True))
-  (ensures (fun h0 _ h1 ->
-    modifies_none h0 h1
+  (ensures (fun h0 pkae_p h1 ->
+    modifies (Set.singleton rgn) h0 h1
   ))
 
-let registered pkm i = ID.registered pkm.pim i
-let honest pkm i = ID.honest pkm.pim i
-let dishonest pkm i = ID.dishonest pkm.pim i
+//val pkey_length: n32
+let pkey_length = 32
+val pkey : Type
+val get_pkey_raw: pkey -> Tot (lbytes pkey_length)
+val get_pkey_id: pk:pkey -> Tot (i:pk_id{i = PK_id (get_pkey_raw pk)})
 
-val encrypt: pkm:pkae_module ->
-             n:nonce ->
-             sk:skey pkm ->
-             pk:pkey pkm{compatible_keys pkm sk pk} ->
-             m:(Plain.protected_plain_t pkm.pim (Plain.get_plain pkm.pm) (compose_ids pkm (pkey_to_subId #pkm pk) (pkey_to_subId #pkm (pkey_from_skey pkm sk)))) ->
-             ST cipher
+//val skey_length: n32
+let skey_length = 32
+val skey : Type
+val get_skey_raw: skey -> GTot (lbytes pkey_length)
+val get_pkey_from_skey: skey -> pkey
+val get_skey_id: sk:skey -> Tot (i:pk_id{i = PK_id (get_pkey_raw (get_pkey_from_skey sk))})
+
+val gen : #rgn:erid -> ip:index_package rgn -> ST (keypair:(pkey*skey))
+  (requires (fun h0 -> True))
+  (ensures (fun h0 keypair h1 ->
+    get_pkey_from_skey (snd keypair) == fst keypair
+    /\ honest ip (PK_id (get_pkey_raw (fst keypair)))
+    /\ modifies (Set.singleton rgn) h0 h1
+  ))
+
+val coerce : #rgn:erid -> ip:index_package rgn -> pk_raw:lbytes pkey_length -> sk_raw:lbytes skey_length ->ST (keypair:(pkey*skey))
   (requires (fun h0 ->
-    let i = compose_ids pkm (pkey_to_subId #pkm pk) (pkey_to_subId #pkm (pkey_from_skey pkm sk)) in
-    registered pkm i
-    ///\ (Flags.Game0? Flags.current_game \/ Flags.Game5? Flags.current_game)
-    /\ nonce_is_fresh pkm i n h0
-    /\ invariant pkm h0
+    fresh ip (PK_id pk_raw) h0
   ))
-  (ensures  (fun h0 c h1 ->
-    let i = compose_ids pkm (pkey_to_subId #pkm pk) (pkey_to_subId #pkm (pkey_from_skey pkm sk)) in
-    True //modifies (Set.singleton pkm.rgn) h0 h1 // stateful changes even if the id is dishonest.
-    /\ ((honest pkm i /\ b2t pkae) // Ideal behaviour if the id is honest and the assumption holds
-               ==> eq2 #cipher c (enc pkm (zero_bytes (Plain.length #pkm.pim #pkm.pm #i m)) n pk sk))
-    /\ ((dishonest pkm i \/ ~(b2t pkae)) // Concrete behaviour otherwise.
-                  ==> eq2 #cipher c (enc pkm (Plain.repr #pkm.pim #pkm.pm #i m) n pk sk))
-    // The message is added to the log. This also guarantees nonce-uniqueness.
-    /\ MR.m_contains #(get_message_log_region pkm)(get_message_logGT pkm) h1
-    /\ MR.witnessed (MM.contains #(get_message_log_region pkm) (get_message_logGT pkm) (n,i) (c,m))
-    /\ MR.m_sel #(get_message_log_region pkm) h1 (get_message_logGT pkm)== MM.upd (MR.m_sel #(get_message_log_region pkm) h0 (get_message_logGT pkm)) (n,i) (c,m)
-    /\ invariant pkm h1
+  (ensures (fun h0 keypair h1 ->
+    get_pkey_from_skey (snd keypair) == fst keypair
+    /\ dishonest ip (get_pkey_id (fst keypair))
+    /\ get_pkey_raw (fst keypair) = pk_raw
+    /\ get_skey_raw (snd keypair) = sk_raw
+    /\ modifies (Set.singleton rgn) h0 h1
   ))
 
-val decrypt: pkm:pkae_module ->
-             n:nonce ->
-             sk:skey pkm ->
-             pk:pkey pkm{compatible_keys pkm sk pk} ->
-             c:cipher ->
-             ST (option (Plain.protected_plain_t pkm.pim (Plain.get_plain pkm.pm) (compose_ids pkm (pkey_to_subId #pkm pk) (pkey_to_subId #pkm (pkey_from_skey pkm sk)))))
+val compose_ids: pk_id -> pk_id -> inst_id
+
+val nonce_length:n32
+let nonce = lbytes nonce_length
+val valid_ciphertext_length : n32 -> bool
+let ciphertext = b:bytes32{valid_ciphertext_length (Seq.length b)}
+
+val compatible_keys: pkey -> skey -> bool
+
+type message_log_key =
+  | LOG_KEY: i:inst_id -> n:nonce -> c:ciphertext -> message_log_key
+
+let message_log_value (i:inst_id) = protected_plain pp i
+let message_log_range (k:message_log_key) = message_log_value (k.i)
+let message_log_inv (f:MM.map' (message_log_key) (message_log_range)) = True
+
+let message_log (rgn:erid) =
+  MM.t rgn (message_log_key) (message_log_range) (message_log_inv)
+
+val get_log: #rgn:erid -> pkae_package rgn -> message_log rgn
+
+let nonce_is_unique (#rgn:erid) (pkae_p:pkae_package rgn) (i:inst_id) (n:nonce) (h0:mem) =
+  forall c . MM.fresh (get_log pkae_p) (LOG_KEY i n c) h0
+
+let extended_message_log (#rgn:erid) (pkae_p:pkae_package rgn) (i:inst_id) (n:nonce) (c:ciphertext) (p:protected_plain pp i) (h0:mem) (h1:mem) =
+  let log_key = LOG_KEY i n c in
+  let log_value = p in
+  let log = get_log pkae_p in
+  sel h1 log == MM.upd (sel h0 log) log_key log_value
+  /\ witnessed (MM.defined log log_key)
+  /\ witnessed (MM.contains log log_key log_value)
+
+
+val enc_spec: p:plain pp -> pk:lbytes pkey_length -> sk:lbytes skey_length -> n:nonce -> c:ciphertext
+val enc_star: plain_length:n32 -> pk:lbytes pkey_length -> sk:lbytes skey_length -> n:nonce -> c:ciphertext
+val dec_spec: c:ciphertext -> pk:lbytes pkey_length -> sk:lbytes skey_length -> n:nonce -> option (p:plain pp)
+
+#set-options "--z3rlimit 300 --max_ifuel 0 --max_fuel 0"
+val encrypt: #rgn:erid -> pkae_p:pkae_package rgn -> ip:index_package rgn -> pk:pkey -> sk:skey{compatible_keys pk sk} -> n:nonce -> p:protected_plain pp (compose_ids (get_pkey_id pk) (get_skey_id sk)) -> ST ciphertext
   (requires (fun h0 ->
-    let i = compose_ids pkm (pkey_to_subId #pkm pk) (pkey_to_subId #pkm (pkey_from_skey pkm sk)) in
-    registered pkm i
-    /\ invariant pkm h0
+    let i = compose_ids (get_pkey_id pk) (get_skey_id sk) in
+    nonce_is_unique pkae_p i n h0
   ))
-  (ensures  (fun h0 p h1 ->
-    let i = compose_ids pkm (pkey_to_subId #pkm pk) (pkey_to_subId #pkm (pkey_from_skey pkm sk)) in
-    h0 == h1
-    /\ invariant pkm h1
-    /\ ((~(b2t pkae) \/ dishonest pkm i) ==> // Concrete behaviour of the id is dishonest or if the assumption doesn't hold.
-        (let option_m = dec pkm c n pk sk in // Functional correctness: we get a result iff the ciphertext is valid.
-        (Some? option_m ==>
-          Some? p /\ Some?.v p == Plain.make_prot_plainGT #pkm.pim #pkm.pm #i (Some?.v option_m))
-        /\ (None? option_m ==>
-            None? p)
-      ))
-    /\ (let log = get_message_logGT pkm in
-      (b2t pkae /\ honest pkm i) ==> // Ideal behaviour otherwise: We get a result iff something is in the log.
-        (Some? p ==>
-          (MM.defined log (n,i) h0 /\ (fst (MM.value log (n,i) h0) == c )
-          /\ Some?.v p == snd (MM.value log (n,i) h0)))
-      /\ (None? p ==>
-          (MM.fresh log (n,i) h0 \/ c =!= fst (MM.value log (n,i) h0)))
-    )
+  (ensures (fun h0 c h1 ->
+    let i = compose_ids (get_pkey_id pk) (get_skey_id sk) in
+    //let both_honest = honest ip i in
+    modifies (Set.singleton rgn) h0 h1
+    /\ ((honest ip i /\ pkae_flag) ==>
+      c == enc_star (length p) (get_pkey_raw pk) (get_skey_raw sk) n)
+    /\ ((dishonest ip i \/ ~(b2t pkae_flag)) ==>
+      c == enc_spec (repr #rgn #pp #ip #i p) (get_pkey_raw pk) (get_skey_raw sk) n)
+    /\ extended_message_log pkae_p i n c p h0 h1
+  ))
+
+val decrypt: #rgn:erid -> pkae_p:pkae_package rgn -> ip:index_package rgn -> pk:pkey -> sk:skey{compatible_keys pk sk} -> n:nonce -> c:ciphertext -> ST (option_p:option (protected_plain pp (compose_ids (get_pkey_id pk) (get_skey_id sk))))
+  (requires (fun h0 ->
+    True
+  ))
+  (ensures (fun h0 option_p h1 ->
+    let i = compose_ids (get_pkey_id pk) (get_skey_id sk) in
+    let option_spec = dec_spec c (get_pkey_raw pk) (get_skey_raw sk) n in
+    (modifies (Set.singleton rgn) h0 h1 \/ h0 == h1)
+    /\ ((honest ip i /\ pkae_flag) ==>
+      (MM.sel (sel h0 (get_log pkae_p)) (LOG_KEY i n c) == option_p)
+      )
+    /\ ((dishonest ip i \/ ~(b2t pkae_flag)) ==>
+      (Some? option_spec ==>
+      (Some? option_p
+      /\ repr #rgn #pp #ip #i (Some?.v option_p) == Some?.v option_spec))
+      )
   ))
