secure_api/box/Box.Plain.fst
@@ -1,102 +1,31 @@
-(**
-  This module contains the plaintext type of AE and functions to access it.
-*)
 module Box.Plain
 
-open FStar.Seq
-open FStar.HyperHeap
+open Box.Key
+open Box.Index
+
+open FStar.Endianness
 open FStar.HyperStack
 open FStar.HyperStack.ST
 
-open Box.Flags
-open Box.Index
+let n32 = (n:nat{n<=32})
 
-(**
-  The protected plaintext type of AE. It is associated with an id and acts as a wrapper around a protected pkae plaintext.
-  The ids associated with both plaintexts must be equal.
-*)
+noeq type plain_package =
+  | PP:
+    flag:Type0 ->
+    valid_length:(n32 -> bool) ->
+    plain_package
 
-#set-options "--z3rlimit 300 --max_ifuel 1 --max_fuel 0"
-abstract noeq type plain_module =
-  | PM:
-    plain: Type0 ->
-    //repr: ((#i:id im) -> (protected_plain_t i) -> (p:plain_type{dishonest im (ID i) \/ not ae_ind_cpa})) ->
-    //coerce: (#i:id im -> plain_type -> (p:protected_plain_t i{dishonest im (ID i) \/ not ae_int_ctxt})) ->
-    valid_length: (nat -> bool)->
-    length: (plain -> n:nat{valid_length n}) ->
-    plain_module
+type plain (pp:plain_package) = p:bytes{Seq.length p <= 32 /\ pp.valid_length (Seq.length p)}
+abstract type protected_plain (pp:plain_package) (i:inst_id) = plain pp
 
-abstract type protected_plain_t (im:index_module) (pt:Type0) (id:id im) = pt
+val length: (#pp:plain_package) -> (#i:inst_id) -> (p:protected_plain pp i) -> n:n32{pp.valid_length n}
+let length #pp #i p =
+  Seq.length p
 
-val lemma_index_module: im:index_module -> i:id im -> ST unit
-  (requires (fun h0 -> registered im i))
-  (ensures (fun h0 _ h1 ->
-    (honest im i ==> (~(dishonest im i)))
-    /\ (dishonest im i ==> (~(honest im i)))
-  ))
-
-let lemma_index_module im i =
-  lemma_index_module im i
-
-val get_plain: pm:plain_module -> (t:Type0{t == pm.plain})
-let get_plain pm =
-  pm.plain
-
-
-val make_plainGT: #im:index_module -> #pm:plain_module -> #i:id im -> protected_plain_t im pm.plain i -> GTot (p:pm.plain)
-let make_plainGT #im #pm #i p =
+val coerce: (#rgn:erid) -> (#pp:plain_package) -> ip:index_package rgn -> (i:inst_id{dishonest ip i \/ ~pp.flag}) -> p:plain pp -> p:protected_plain pp i
+let coerce #pp #rgn i ip p =
   p
 
-val repr: #im:index_module -> #pm:plain_module -> #i:id im{dishonest im i \/ not ae_ind_cpa} -> protected_plain_t im pm.plain i -> (p:pm.plain)
-let repr #im #pm #i p =
-  p
-
-val make_prot_plainGT: #im:index_module -> #pm:plain_module -> #i:id im -> p:pm.plain -> GTot (protected_plain_t im pm.plain i)
-let make_prot_plainGT #im #pm #i p =
-  p
-
-val coerce: #im:index_module -> #pm:plain_module -> #i:id im{dishonest im i \/ not ae_int_ctxt} -> pm.plain -> (p:protected_plain_t im pm.plain i)
-let coerce #im #pm #i p =
-  p
-
-val valid_length: #pm:plain_module -> n:nat -> b:bool//{b=pm.valid_length n}
-let valid_length #pm n = pm.valid_length n
-
-val lemma_valid_length: pm:plain_module -> Lemma (requires True) (ensures pm.valid_length == valid_length #pm) [SMTPat (valid_length #pm)]
-let lemma_valid_length pm =
-  assert (FStar.FunctionalExtensionality.feq (pm.valid_length) (valid_length #pm));
-  ()
-
-val create: plain:Type0 ->
-            pm_valid_length:(nat -> bool) ->
-            length:(plain ->
-            n:nat{pm_valid_length n}) ->
-            pm:plain_module{
-              pm.plain==plain
-              /\ get_plain pm == plain
-              /\ valid_length #pm == pm_valid_length
-              /\ pm.valid_length == pm_valid_length
-              /\ pm.length==length}
-let create plain valid_length length =
-  PM plain valid_length length
-
-val length: #im:index_module -> #pm:plain_module -> #i:id im -> (p:protected_plain_t im pm.plain i) -> n:nat{n=pm.length p /\ pm.valid_length n}
-let length #im #pm #i p =
-  pm.length p
-
-val rec_repr: #im:index_module ->
-              #inner_pm:plain_module ->
-              #pm:plain_module ->
-              #i:id im{dishonest im i \/ not ae_ind_cpa} ->
-              p:protected_plain_t im pm.plain i{protected_plain_t im pm.plain i === protected_plain_t im inner_pm.plain i}
-              -> Tot (inner_pm.plain)
-let rec_repr #im #inner_pm #pm #i p =
-  repr #im #inner_pm #i p
-
-val message_wrap: #im:index_module -> #inner_pm:plain_module -> #pm:plain_module -> #i:id im -> p:inner_pm.plain{protected_plain_t im pm.plain i === protected_plain_t im inner_pm.plain i} -> protected_plain_t im pm.plain i
-let message_wrap #im #inner_pm #pm #i p =
-  p
-
-val message_unwrap: #im:index_module -> #inner_pm:plain_module -> #pm:plain_module -> #i:id im -> p:pm.plain{protected_plain_t im pm.plain i === protected_plain_t im inner_pm.plain i} -> protected_plain_t im inner_pm.plain i
-let message_unwrap #im #inner_pm #pm #i p =
+val repr: (#rgn:erid) -> (#pp:plain_package) -> #ip:index_package rgn -> (#i:inst_id{dishonest ip i \/ ~pp.flag}) -> p:protected_plain pp i -> p:plain pp
+let repr #rgn #pp #ip #i p =
   p
