secure_api/box/Box.Flags.fsti
@@ -1,72 +1,7 @@
-(**
-   This module contains flags that control the idealization of encryption and decryption,
-   both of AE and of PKE. The flags indicate whether certain assumption are assumed to be
-   true or not. Also, the refinements on the flag type indicate implications between the
-   assumptions such as ae_ind_cpa /\ ae_int_ctxt ==> ae_ind_cca.
-   Note, that for purposes of type-checking, the flags are not set. This
-   ensures that the program is well typed for any permutation of set flags (that is permissible
-   by the refinements).
-*)
 module Box.Flags
 
+val prf_odh : b:bool
 
-// Flags representing steps/games in the proof.
-type game =
-  | Game0
-  | Game1
-  | Game2
-  | Game3
-  | Game4
-  | Game5
+val ae: b:bool{b ==> prf_odh}
 
-(** The current game step indicates which modules are currently idealized,
-    not idealized or for which modules idealization is not fixed.
-    For the exact state of the game at each step, see the individual flags
-    below.
-*)
-val current_game : g:game
-//{
-//  match g with
-//  | Game0 -> not ae_ind_cpa /\ ~ae_int_ctxt /\ ~prf_odh /\ not pkae
-//  | Game1 -> not ae_ind_cpa /\ ~ae_int_ctxt /\ not pkae
-//  | Game2 -> prf_odh /\ not pkae
-//  | Game3 -> b2t ae_ind_cca /\ prf_odh /\ not pkae
-//  | Game4 -> b2t ae_ind_cca /\ not pkae
-//  | Game5 -> b2t ae_ind_cca /\ ~prf_odh /\ b2t pkae
-//  }
-
-val prf_odh : b:bool{(Game0? current_game ==> ~b)
-                     /\ (Game1? current_game ==> (b \/ ~b))
-                     /\ (Game2? current_game ==> b)
-                     /\ (Game3? current_game ==> b)
-                     /\ (Game4? current_game ==> (b \/ ~b))
-                     /\ (Game5? current_game ==> ~b)
-                     }
-
-val ae_int_ctxt : b:bool{(Game0? current_game ==> ~b)
-                         /\ (Game1? current_game ==> ~b)
-                         /\ (Game2? current_game ==> (b \/ ~b))
-                         /\ (Game3? current_game ==> b)
-                         /\ (Game4? current_game ==> b)
-                         /\ (Game5? current_game ==> b)
-                         }
-
-val ae_ind_cpa : b:bool{(Game0? current_game ==> ~b)
-                        /\ (Game1? current_game ==> ~b)
-                        /\ (Game2? current_game ==> (b \/ ~b))
-                        /\ (Game3? current_game ==> b)
-                        /\ (Game4? current_game ==> b)
-                        /\ (Game5? current_game ==> b)
-                        }
-
-val ae_ind_cca : b:bool{(Game0? current_game ==> ~b)
-                        /\ (Game1? current_game ==> ~b)
-                        /\ (Game2? current_game ==> (b \/ ~b))
-                        /\ (Game3? current_game ==> b)
-                        /\ (Game4? current_game ==> b)
-                        /\ (Game5? current_game ==> b)
-                        }
-
-val pkae : b:bool{(Game0? current_game <==> ~b)
-                  /\ (Game5? current_game <==> b)
-                  }
+val pkae : b:bool{b ==> prf_odh /\ ae}
